almost working example with unknown expr

theories/simplang/na_inv/examples/data_races.v
@@ -1,9 +1,10 @@
-From simuliris.simplang Require Import lang notation tactics class_instances proofmode gen_log_rel.
+From simuliris.simplang Require Import lang notation tactics class_instances proofmode gen_log_rel parallel_subst wf.
 From iris Require Import bi.bi.
 Import bi.
 From iris.proofmode Require Import tactics.
 From simuliris.simulation Require Import slsls lifting.
 From simuliris.simplang.na_inv Require Export inv.
+From simuliris.simplang.na_inv Require Import readonly_refl.
 
 (** * Examples for exploiting UB of data-races. *)
 
@@ -32,7 +33,7 @@ Section data_race.
     ⊢ log_rel remove_store_and_load_opt remove_store_and_load.
   Proof.
     log_rel.
-    iIntros "%v2_t %v2_s #Hv2 %v1_t %v1_s #Hv1 !# %π Hc".
+    iIntros "%v2_t %v2_s #Hv2 %v1_t %v1_s #Hv1 !# %π Hc". simpl_subst.
 
     sim_bind (! _)%E (! _)%E. iApply sim_irred_unless; first done. iIntros ([l1_s ->]).
     iPoseProof (gen_val_rel_loc_source with "Hv1") as (l_t1 ->) "#Hl1".
@@ -78,29 +79,29 @@ Section data_race.
     log_rel.
   Abort.
 
-  Definition hoist_load_opt : expr :=
-     if: "n" < #1 then
-       #0
-     else
-       let: "mval" := !"m" in
-       let: "r" := ref "mval" in
-       let: "i" := ref #1 in
-       while: ! "i" < "n" do
-         "r" <- !"r" + "mval";;
-         (* Call f#fname "x";; *)
-         "i" <- !"i" + #1
-       od;;
-       Free "i";;
-       let: "res" := !"r" in
-       Free "r";;
-       "res".
+  Definition hoist_load_opt (e : expr) : expr :=
+    let: "i" := ref #0 in
+    if: e then
+      let: "mval" := !"m" in
+      let: "r" := ref "mval" in
+      "i" <- !"i" + #1;;
+      while: e do
+        "r" <- !"r" + "mval";;
+        "i" <- !"i" + #1
+      od;;
+      Free "i";;
+      let: "res" := !"r" in
+      Free "r";;
+      "res"
+    else
+      Free "i";;
+      #0.
 
-  Definition hoist_load : expr :=
+  Definition hoist_load (e : expr) : expr :=
      let: "r" := ref #0  in
      let: "i" := ref #0  in
-     while: ! "i" < "n" do
+     while: e do
        "r" <- !"r" + !"m";;
-       (* Call f#fname "x";; *)
        "i" <- !"i" + #1
      od;;
      Free "i";;
@@ -108,40 +109,47 @@ Section data_race.
      Free "r";;
      "res".
 
-  Lemma hoist_load_sim:
-    ⊢ log_rel hoist_load_opt hoist_load.
+  Lemma hoist_load_sim e:
+    free_vars e = list_to_set ["n"; "i"] →
+    gen_expr_wf readonly_wf e →
+    ⊢ log_rel (hoist_load_opt e) (hoist_load e).
   Proof.
-    log_rel.
+    move => He ?. log_rel.
     iIntros "%v_t1 %v_s1 #Hrel1 %v_t2 %v_s2 #Hrel2 !# %π Hc".
 
     source_alloc lr_s as "Hlr_s" "Hfr_s". sim_pures.
     source_alloc li_s as "Hli_s" "Hfi_s". sim_pures.
-    source_while. source_load.
-    source_bind (_ < _)%E. iApply source_red_irred_unless; first done.
-    iIntros ([[??] [??]]); simplify_eq.
-    iDestruct (gen_val_rel_litint_source with "Hrel2") as %->. sim_pures. sim_pures.
-    case_bool_decide; [rewrite bool_decide_false;[|lia]|rewrite bool_decide_true;[|lia]]; sim_pures.
-    - source_free. sim_pures. source_load. sim_pures. source_free. sim_pures. by sim_val; iFrame.
+    target_alloc li_t as "Hli_t" "Hfi_t". sim_pures.
+    source_while. to_sim.
+    sim_bind (subst_map _ _) (subst_map _ _).
+    iApply (sim_refl with "[] [Hc]");
+      [compute_done | rewrite He; compute_done
+       | apply: readonly_log_rel_structural [] ∅ | done | | |].
+    { admit. }
+    { iFrame. unfold mapsto_list, na_locs_in_mapsto_list. iSplit; [|done]. iPureIntro. set_solver. }
+    iIntros (v_t v_s) "(_ & Hc & _) Hv". iApply lift_post_val.
+    source_bind (If _ _ _). discr_source. val_discr_source "Hv".
+    revert select (bool) => -[]; sim_pures; sim_pures; last first.
+    - target_free. source_free. sim_pures. source_load. source_free. sim_pures. sim_val. by iFrame.
     - source_bind (! _)%E. iApply source_red_irred_unless; first done.
       iIntros ([l_s ?]); simplify_eq.
       iDestruct (gen_val_rel_loc_source with "Hrel1") as (l_t ->) "Hbij".
-      do 2 iApply source_red_base. do 2 iModIntro.
+      do 3 iApply source_red_base. do 3 iModIntro.
       iApply (sim_bij_exploit_load with "Hbij Hc"); [|done|]. {
         intros. reach_or_stuck_fill (! _)%E => /=.
         apply: reach_or_stuck_refl. apply: post_in_ectx_intro. naive_solver.
       }
       iIntros (q v_t v_s) "Hl_t Hl_s #Hv Hc".
-      iDestruct (heap_mapsto_ne with "Hlr_s Hli_s") as %Hne1.
+      iApply sim_update_si. iApply (sim_bij_freeable_ne with "Hbij Hfr_s"). iIntros (Hne1) "Hfr_s".
+      iApply sim_update_si. iApply (sim_bij_freeable_ne with "Hbij Hfi_s"). iIntros (Hne3) "Hfi_s".
       iDestruct (heap_mapsto_ne with "Hlr_s Hl_s") as %Hne2.
-      iDestruct (heap_mapsto_ne with "Hli_s Hl_s") as %Hne3.
       source_load. sim_pures. source_load. sim_pures.
       source_bind (_ + _)%E. iApply source_red_irred_unless; first done.
       iIntros ([[??] [m ?]]); simplify_eq.
       iDestruct (gen_val_rel_litint_source with "Hv") as %->. sim_pures. rewrite Z.add_0_l.
       source_store. source_load. source_store. sim_pures.
 
-      target_load. target_alloc lr_t as "Hlr_t" "Hfr_t". target_alloc li_t as "Hli_t" "Hfi_t".
-      sim_pures.
+      target_load. target_alloc lr_t as "Hlr_t" "Hfr_t". target_load. target_store. sim_pures.
       iApply (sim_bij_insert with "Hfi_t Hfi_s Hli_t Hli_s []"); [done|]. iIntros "#Hbiji".
       iApply (sim_bij_insert with "Hfr_t Hfr_s Hlr_t Hlr_s []"); [done|]. iIntros "#Hbijr".
       sim_bind (While _ _) (While _ _).
@@ -149,41 +157,43 @@ Section data_race.
          l_t ↦t{#q} #m ∗ l_s ↦s{#q} #m ∗ na_locs π (<[l_s:=(l_t, NaRead q)]> ∅))%I with "[-]").
       { eauto with iFrame. }
       iIntros "!> (Hl_t&Hl_s&Hc)".
-      sim_bind (! _)%E (! _)%E.
-      iApply (sim_bij_load_na with "Hbiji Hc"); [by simplify_map_eq|].
-      iIntros (??) "Hv' Hc". sim_val.
-      source_bind (_ < _)%E. iApply source_red_irred_unless; first done.
-      iIntros ([[??] [??]]); simplify_eq.
-      iDestruct (gen_val_rel_litint_source with "Hv'") as %->. sim_pures. sim_pures.
-      case_bool_decide; sim_pures.
+      sim_bind (subst_map _ _) (subst_map _ _).
+      iApply (sim_refl with "[] [Hc Hl_t Hl_s]");
+        [compute_done | rewrite He; compute_done
+         | apply (readonly_log_rel_structural [(l_t, l_s, #m ,#m , q)]) | done | | |]. {
+        rewrite !dom_insert_L. iApply big_sepS_intro. iIntros "!#" (x Hin).
+        rewrite map_lookup_zip_with.
+        destruct (decide (x = "n")); [| destruct (decide (x = "i")); [|exfalso; set_solver]]; by simplify_map_eq.
+      } {
+        iFrame "∗ Hrel1". iSplit; [| by eauto ]. iPureIntro.
+        move => ??? /lookup_insert_Some[[??]|[??]]; simplify_eq. by eexists 0, _, _.
+      }
+      iIntros (??) "(_ & Hc & Hm) Hb". rewrite /mapsto_list /=. iApply lift_post_val.
+      iDestruct "Hm" as "[(Hl_t & Hl_s & _ & _) _]".
+      discr_source. val_discr_source "Hb".
+      revert select (bool) => -[]; sim_pures.
       + source_load. sim_pures.
         sim_bind (! _)%E (! _)%E.
         iApply (sim_bij_load_na with "Hbijr Hc"); [by simplify_map_eq|].
         iIntros (??) "Hv'' Hc". sim_val.
-        source_bind (_ + _)%E. iApply source_red_irred_unless; first done.
-        iIntros ([[??] [??]]); simplify_eq.
-        iDestruct (gen_val_rel_litint_source with "Hv''") as %->. sim_pures. sim_pures.
+        source_bind (_ + _)%E. discr_source. val_discr_source "Hv''"; simplify_eq. sim_pures. sim_pures.
         sim_bind (_ <- _)%E (_ <- _)%E.
         iApply (sim_bij_store_na with "Hbijr Hc"); [by simplify_map_eq| done |].
         iIntros "Hc". sim_val. sim_pures.
 
         sim_bind (! _)%E (! _)%E.
-        iApply (sim_bij_load_na with "Hbiji Hc"); [by simplify_map_eq|].
+        iApply (sim_bij_load_na with "Hbiji Hc"); [admit|].
         iIntros (??) "Hv''' Hc". sim_val.
-        source_bind (_ + _)%E. iApply source_red_irred_unless; first done.
-        iIntros ([[??] [??]]); simplify_eq.
-        iDestruct (gen_val_rel_litint_source with "Hv'''") as %->. sim_pures. sim_pures.
+        source_bind (_ + _)%E. discr_source. val_discr_source "Hv'''"; simplify_eq. sim_pures. sim_pures.
         sim_bind (_ <- _)%E (_ <- _)%E.
-        iApply (sim_bij_store_na with "Hbiji Hc"); [by simplify_map_eq| done |].
+        iApply (sim_bij_store_na with "Hbiji Hc"); [admit | done |].
         iIntros "Hc". sim_val. sim_pures.
 
         iApply sim_expr_base. iRight. by iFrame.
       + iApply sim_expr_base. iLeft. iApply lift_post_val.
-        sim_pures.
-        sim_bind (FreeN _ _)%E (FreeN _ _)%E.
+        sim_pures. sim_bind (FreeN _ _)%E (FreeN _ _)%E.
         iApply (sim_bij_free with "Hbiji Hc"). {
-          move => i ?. rewrite lookup_insert_ne //.
-          destruct (decide (i = 0%Z)); [subst |lia]. by rewrite loc_add_0.
+          move => i ?. rewrite lookup_insert_ne //. by destruct l_s, li_s => -[??].
         }
         iIntros "Hc". sim_val. sim_pures.
         sim_bind (! _)%E (! _)%E.
@@ -198,7 +208,7 @@ Section data_race.
         iApply (sim_bij_release (NaRead _) with "Hbij Hc [$] [$] Hv"); [by simplify_map_eq| ].
         iIntros "Hc". rewrite delete_insert //.
         sim_val. sim_pures. sim_val; by iFrame.
-  Qed.
+  Abort.
 
   (* TODO: try also other direction (or maybe another example that adds loads and that makes more sense) *)
 
