theories/simplang/gen_log_rel.v
@@ -232,4 +232,27 @@ Section log_rel_structural.
     all: iApply gen_log_rel_refl; [done|].
     all: naive_solver.
   Qed.
+
+  Corollary sim_refl π m1 m2 e Φ :
+    dom (gset _) m1 = dom (gset _) m2 →
+    free_vars e = dom (gset _) m1 →
+    log_rel_structural →
+    gen_expr_wf expr_head_wf e →
+    subst_map_rel loc_rel (dom _ m1) (map_zip m1 m2) -∗
+    thread_own π -∗
+    (∀ v_t v_s, thread_own π -∗ gen_val_rel loc_rel v_t v_s -∗ Φ (Val v_t) (Val v_s)) -∗
+    subst_map m1 e ⪯{π} subst_map m2 e [{ Φ }].
+  Proof.
+    iIntros (Hdom Hfree ??) "Hrel Ht HΦ".
+    iApply (sim_expr_wand with "[Hrel Ht]").
+    - iPoseProof gen_log_rel_refl as "#Hlog"; [done..|].
+      iSpecialize ("Hlog" $! _ (map_zip m1 m2)).
+      setoid_rewrite fst_map_zip.
+      2: { move => ?. by rewrite -!elem_of_dom Hdom. }
+      setoid_rewrite snd_map_zip.
+      2: { move => ?. by rewrite -!elem_of_dom Hdom. }
+      iApply ("Hlog" with "[Hrel] Ht"). by rewrite Hfree idemp_L.
+    - iIntros (e_t e_s) "(%v_t & %v_s & -> & -> & Ht & Hv)". by iApply ("HΦ" with "Ht").
+  Qed.
+
 End log_rel_structural.
